more

thys/Common_Rec_Corec/Bimodels_are_Models.thy
@@ -7,19 +7,21 @@ begin
 context Bimodel 
 begin 
 
-
-definition EEctor' :: "('a::var,'a,'a P\<Rightarrow>'a E','a P\<Rightarrow>'a E') G \<Rightarrow> 'a P\<Rightarrow>'a E'" where 
+ 
+(* definition EEctor' :: "('a::var,'a,'a P\<Rightarrow>'a E','a P\<Rightarrow>'a E') G \<Rightarrow> 'a P\<Rightarrow>'a E'" where 
 "EEctor' u \<equiv> if base u then Ector' u else Ector' u"
+*)
 
-lemma EEctor'_base[simp]: "base u \<Longrightarrow> EEctor' u = Ector' u"
+(* lemma EEctor'_base[simp]: "base u \<Longrightarrow> EEctor' u = Ector' u"
 unfolding EEctor'_def by auto
 
 lemma EEctor'_step[simp]: "\<not> base u \<Longrightarrow> EEctor' u = Ector' u"
-unfolding EEctor'_def by auto
+unfolding EEctor'_def by auto *)
 
-lemma ctorPermM: "ctorPermM EEctor' Eperm u"
+(*
+lemma ctorPermM: "ctorPermM Ector' Eperm u"
 unfolding ctorPermM_def apply safe
-  subgoal for \<sigma> apply(cases "base u")
+  subgoal for \<sigma> apply(cases "base u") 
     subgoal unfolding EEctor'_base  
     apply(subst ctorPermM_Ector'[unfolded ctorPermM_def, rule_format])
       subgoal by auto
@@ -42,13 +44,13 @@ unfolding ctorVarsM_def
     subgoal unfolding EEctor'_step apply(intro allI impI) 
     apply(rule subset_trans[OF ctorVarsM_Ector'[unfolded ctorVarsM_def, rule_format]]) 
     using base_Gmap by auto . 
+*)
 
 
 (* models from special_models: *)
-sublocale M : Model where Ector' = EEctor' and Eperm' = Eperm and EVrs' = EVrs 
+sublocale M : Model where Ector' = Ector' and Eperm' = Eperm and EVrs' = EVrs 
 apply standard 
-using nom ctorPermM ctorVarsM by auto   
-
+using nom ctorPermM_Ector' ctorVarsM_Ector' ctor_compat_Pvalid_Ector' by auto
 
 (* Borrowing the recursion from models, under the assumption that E 
 is inital; I essentially copy the recursor, and I customize it a bit 
@@ -60,6 +62,13 @@ and extract the same recursion principle from corecursion/finality.) *)
 thm M.rec_Ector M.rec_Eperm M.rec_unique M.rec_EVrs[no_vars] M.rec_Eperm[no_vars]
 definition "mrec \<equiv> M.rec"
 
+(* TODO: go back to Ector'', take advantage of its simpler nature *)
+
+theorem mrec_Ector_base:
+assumes "base u"    
+and "Pvalid p" and "GVrs2 u \<inter> PVrs p = {}" and "GVrs2 u \<inter> GVrs1 u = {}"
+shows "mrec (Ector u) p = Ector' (Gmap mrec mrec u) p" 
+
 theorem mrec_Ector_base:
 assumes "base u"    
 and "Pvalid p" and "GVrs2 u \<inter> PVrs p = {}" and "GVrs2 u \<inter> GVrs1 u = {}"
@@ -68,10 +77,8 @@ unfolding mrec_def
 apply(subst M.rec_Ector) 
   subgoal using assms by simp
   subgoal using assms by simp
-  subgoal using assms by simp
-  subgoal using assms apply(subst EEctor'_base)
-    subgoal using base_Gmap by blast
-    subgoal unfolding Gmap_comp unfolding o_def by simp . .
+  subgoal using assms by simp  
+  subgoal by simp . 
 
 theorem mrec_Ector_step:
 assumes "\<not> base u" 
